updates to bezout and q3 - WIP!!

q3.dfy
@@ -14,13 +14,33 @@ predicate divides(a: nat, b: nat)
     exists c :: b == c * a
 }
 
+predicate quotientRemainderPredicate(a: nat, b: nat, q: nat, r: nat)
+{
+    a == (q * b) + r && 0 <= r < b
+}
+
+lemma quotientRemainder(a: nat, b: nat)
+    requires b > 0
+    ensures exists q, r :: quotientRemainderPredicate(a, b, q, r)
+{
+    if a == 0 
+    {
+        assert quotientRemainderPredicate(a, b, 0, 0);
+    }
+    else
+    {
+        assert a > 0;
+        quotientRemainder(a - 1, b);
+
+    }
+}
+
 // Bezout identity lemma
 lemma bezout(p: nat, q: nat, x: int, y: int)
     requires p != 0 && q != 0 
     ensures p*x + q*y == gcd(p,q)
 {
     // Proof of lemma
-    
 }
 
 lemma corectness(a: nat, b: nat, c: nat)
